demos/sha256/SHA256_Int_AST_Output.v
@@ -1,0 +1,33 @@
+Require Import oeuf.Common.
+
+Require Import oeuf.HList.
+Require Import oeuf.Utopia.
+Require Import oeuf.SourceLifted oeuf.SourceValues.
+Require Import oeuf.CompilationUnit.
+
+Require Import NArith.
+
+Require Import SHA256_Int_AST.
+
+Require Import OeufPlugin.OeufPlugin.
+
+
+Require Import oeuf.Pretty.
+From PrettyParsing Require Import PrettyParsing.
+
+
+Require Import String.
+Require Import Ascii.
+
+Require Import compcert.lib.Integers.
+
+
+(* Without this, `compute` will avoid unfolding `Int.repr`, and then spin out
+ * computing in useless parts of the tree. *)
+Transparent Int.repr.
+
+Time Definition sha_256_tree :=
+    Eval compute in Pretty.compilation_unit.to_tree sha_256_cu.
+
+Time Oeuf Eval lazy Then Write To File "sha256_int.oeuf"
+     (print_tree sha_256_tree).
